Start moving arithmetic lemmas from zeta into cpp2v-core

theories/lang/cpp/semantics/builtins.v
@@ -44,37 +44,452 @@ Definition trailing_zeros (sz : bitsize) (n : Z) : Z :=
 Definition leading_zeros (sz : bitsize) (l : Z) : Z :=
   bitsZ sz - Z.log2 (l mod (2^64)).
 
+(* TODO: using bool_decide would simplify this reasoning. *)
+#[local] Ltac churn_bits :=
+  repeat match goal with
+  | |- context[(?l <=? ?r)%Z] =>
+    let Hnb := fresh "Hnb" in
+    let Hn := fresh "Hn" in
+    destruct (l <=? r)%Z eqn:Hnb;
+      set (Hn := Hnb);
+      [ apply Z.leb_le in Hn
+      | apply Z.leb_gt in Hn]
+  | |- context[(?l <? ?r)%Z] =>
+    let Hnb := fresh "Hnb" in
+    let Hn := fresh "Hn" in
+    destruct (l <? r)%Z eqn:Hnb;
+      set (Hn := Hnb);
+      [ apply Z.ltb_lt in Hn
+      | apply Z.ltb_ge in Hn]
+  end; rewrite ?andb_false_l ?andb_false_r ?andb_true_l ?andb_true_r
+               ?orb_false_l ?orb_false_r ?orb_true_l ?orb_true_r ?Z.bits_0 //=;
+               try lia.
 
-Local Definition bswap16 (n : Z) : Z :=
-  Z.lor (Z.shiftl (Z.land n 255) 8) (Z.land (Z.shiftr n 8) 255).
-Local Definition bswap32 (n : Z) : Z :=
-  let low := bswap16 n in
-  let high := bswap16 (Z.shiftr n 16) in
-  Z.lor (Z.shiftl low 16) high.
-Local Definition bswap64 (n : Z) : Z :=
-  let low := bswap32 n in
-  let high := bswap32 (Z.shiftr n 32) in
-  Z.lor (Z.shiftl low 32) high.
-Local Definition bswap128 (n : Z) : Z :=
-  let low := bswap64 n in
-  let high := bswap64 (Z.shiftr n 64) in
-  Z.lor (Z.shiftl low 64) high.
+Section Byte.
+  Definition _get_byte (x: Z) (n: nat): Z := Z.land (x ≫ (8 * n)) (Z.ones 8).
+  Definition _set_byte (x: Z) (n: nat): Z := (Z.land (Z.ones 8) x) ≪ (8 * n).
 
-Definition bswap (sz : bitsize) : Z -> Z :=
-  match sz with
-  | W8 => id
-  | W16 => bswap16
-  | W32 => bswap32
-  | W64 => bswap64
-  | W128 => bswap128
-  end.
+  Section Theory.
+    Lemma _get_byte_0:
+      forall (idx: nat),
+        _get_byte 0 idx = 0.
+    Proof. intros; by rewrite /_get_byte Z.shiftr_0_l Z.land_0_l. Qed.
 
-Local Definition bytes (ls : list Z) :=
-  fold_left (fun a b => a * 256 + b)%Z ls 0%Z.
-Arguments bytes _%Z.
+    Lemma _set_byte_0:
+      forall (idx: nat),
+        _set_byte 0 idx = 0.
+    Proof. intros; by rewrite /_set_byte Z.shiftl_0_l. Qed.
 
-Local Definition _bswap16_test : bswap W16 (bytes (1::2::nil)%Z) = bytes (2::1::nil)%Z := eq_refl.
-Local Definition _bswap32_test :
-  bswap W32 (bytes (1::2::3::4::nil)%Z) = bytes (4::3::2::1::nil)%Z := eq_refl.
-Local Definition _bswap64_test :
-  bswap W64 (bytes (1::2::3::4::5::6::7::8::nil)%Z) = bytes (8::7::6::5::4::3::2::1::nil)%Z := eq_refl.
+    #[local] Lemma Z_mul_of_nat_S (z : Z) (n : nat) : (z * S n)%Z = (z + z * n)%Z.
+    Proof. lia. Qed.
+
+    Lemma _get_byte_S_idx:
+      forall (v: Z) (idx: nat),
+        _get_byte v (S idx) = _get_byte (v ≫ 8) idx.
+    Proof.
+      intros; rewrite /_get_byte.
+      by rewrite Z.shiftr_shiftr ?Z_mul_of_nat_S; lia.
+    Qed.
+
+    Lemma _get_byte_lor:
+      forall (v v': Z) (idx: nat),
+        _get_byte (Z.lor v v') idx =
+        Z.lor (_get_byte v idx) (_get_byte v' idx).
+    Proof.
+      move=> v v' idx;
+        generalize dependent v;
+        generalize dependent v';
+        induction idx; intros.
+      - rewrite /_get_byte/=.
+        cbv [Z.of_nat Z.mul]; rewrite !Z.shiftr_0_r.
+        by rewrite -Z.land_lor_distr_l.
+      - by rewrite !_get_byte_S_idx Z.shiftr_lor IHidx.
+    Qed.
+
+    Lemma _set_byte_S_idx:
+      forall (v: Z) (idx: nat),
+        _set_byte v (S idx) = ((_set_byte v idx) ≪ 8)%Z.
+    Proof.
+      intros; rewrite /_set_byte.
+      by rewrite Z.shiftl_shiftl ?Z_mul_of_nat_S ?(Z.add_comm 8); lia.
+    Qed.
+
+    Lemma _set_byte_lor:
+      forall (v v': Z) (idx: nat),
+        _set_byte (Z.lor v v') idx =
+        Z.lor (_set_byte v idx) (_set_byte v' idx).
+    Proof.
+      move=> v v' idx;
+        generalize dependent v;
+        generalize dependent v';
+        induction idx; intros.
+      - rewrite /_set_byte/=.
+        cbv [Z.of_nat Z.mul]; rewrite !Z.shiftl_0_r.
+        by rewrite -Z.land_lor_distr_r.
+      - by rewrite !_set_byte_S_idx IHidx Z.shiftl_lor.
+    Qed.
+
+    Lemma _set_byte_shiftl_idx:
+      forall (idx idx': nat) shift v,
+        idx' <= idx ->
+        (shift = 8 * Z.of_nat idx')%Z ->
+        (_set_byte v idx ≫ shift)%Z = _set_byte v (idx - idx').
+    Proof.
+      induction idx; move=> idx' shift v Hidx Hshift.
+      - assert (idx' = 0)%nat by lia; subst.
+        by rewrite Z.shiftr_0_r.
+      - rewrite _set_byte_S_idx; subst.
+        specialize (IHidx (idx' - 1)%nat (8 * Z.of_nat (idx' - 1))%Z v ltac:(lia) eq_refl).
+        destruct idx'.
+        + by rewrite -minus_n_O Z.shiftr_0_r _set_byte_S_idx.
+        + rewrite Z.shiftr_shiftl_r; try lia.
+          rewrite Nat.sub_succ Nat.sub_0_r in IHidx.
+          rewrite Nat.sub_succ -IHidx.
+          repeat f_equal.
+          lia.
+    Qed.
+
+    Lemma _get_byte_nonneg:
+      forall (v: Z) (idx: nat),
+        (0 <= _get_byte v idx)%Z.
+    Proof.
+      intros; rewrite /_get_byte/Z.ones.
+      apply Z.land_nonneg.
+      by right.
+    Qed.
+
+    Lemma _set_byte_nonneg:
+      forall (v: Z) (idx: nat),
+        (0 <= _set_byte v idx)%Z.
+    Proof.
+      intros; rewrite /_set_byte/Z.ones Z.shiftl_nonneg.
+      apply Z.land_nonneg.
+      by left.
+    Qed.
+
+    Lemma _set_byte_land_no_overlap:
+      forall (idx idx': nat) mask v,
+        idx <> idx' ->
+        (mask = Z.ones 8 ≪ (8 * Z.of_nat idx'))%Z ->
+        Z.land (_set_byte v idx) mask = 0.
+    Proof.
+      intros; subst; generalize dependent idx';
+        induction idx; move=> idx' Hidx.
+      - rewrite /_set_byte.
+        apply Z.bits_inj'=> n ?.
+        repeat (rewrite ?Z.lor_spec ?Z.shiftl_spec ?Z.land_spec ?Z.shiftr_spec; try lia).
+        rewrite Z.bits_0 !Z.testbit_ones; try lia.
+        churn_bits.
+      - rewrite /_set_byte.
+        apply Z.bits_inj'=> n ?.
+        repeat (rewrite ?Z.lor_spec ?Z.shiftl_spec ?Z.land_spec ?Z.shiftr_spec; try lia).
+        rewrite Z.bits_0 !Z.testbit_ones; try lia.
+        churn_bits.
+    Qed.
+
+    Lemma _set_byte_land_useless:
+      forall idx mask v,
+        (mask = Z.ones 8 ≪ (8 * Z.of_nat idx))%Z ->
+        Z.land (_set_byte v idx) mask =
+        _set_byte v idx.
+    Proof.
+      intros; subst; induction idx.
+      - rewrite /_set_byte.
+        apply Z.bits_inj'=> n ?.
+        repeat (rewrite ?Z.lor_spec ?Z.shiftl_spec ?Z.land_spec ?Z.shiftr_spec; try lia).
+        rewrite !Z.testbit_ones; try lia.
+        churn_bits.
+        by (replace (n - 8 * Z.of_nat 0)%Z with n by lia).
+      - rewrite /_set_byte.
+        apply Z.bits_inj'=> n ?.
+        repeat (rewrite ?Z.lor_spec ?Z.shiftl_spec ?Z.land_spec ?Z.shiftr_spec; try lia).
+        rewrite !Z.testbit_ones; try lia.
+        churn_bits.
+    Qed.
+
+    Lemma _set_byte_shiftr_big:
+      forall (idx: nat) (idx': Z) v,
+        Z.of_nat idx < idx' ->
+        (_set_byte v idx ≫ (8 * idx'))%Z = 0.
+    Proof.
+      move=> idx idx' v Hidx; generalize dependent idx';
+        induction idx; intros; try lia.
+      - rewrite /_set_byte.
+        apply Z.bits_inj'=> n ?.
+        repeat (rewrite ?Z.lor_spec ?Z.shiftl_spec ?Z.land_spec ?Z.shiftr_spec; try lia).
+        rewrite !Z.testbit_ones; try lia.
+        churn_bits.
+      - rewrite _set_byte_S_idx.
+        rewrite Z.shiftr_shiftl_r; try lia.
+        specialize (IHidx (idx' - 1) ltac:(lia)).
+        by replace (8 * idx' - 8)%Z with (8 * (idx' - 1))%Z by lia.
+    Qed.
+
+    Lemma _get_set_byte_roundtrip:
+      forall (v: Z) (idx idx': nat),
+        idx >= idx' ->
+        _get_byte (_set_byte v idx) idx' = _get_byte v (idx - idx').
+    Proof.
+      move=> v idx idx' Hidx;
+        generalize dependent v;
+        generalize dependent idx';
+        induction idx; intros.
+      - assert (idx' = 0)%nat by lia; subst.
+        rewrite Nat.sub_diag.
+        rewrite /_get_byte/_set_byte/=.
+        cbv [Z.of_nat Z.mul];
+          rewrite ?Z.shiftr_0_r ?Z.shiftl_0_r;
+          try lia.
+        by rewrite Z.land_comm Z.land_assoc Z.land_diag Z.land_comm.
+      - destruct idx'.
+        + rewrite _get_byte_S_idx _set_byte_S_idx -{2}(Nat.sub_0_r idx).
+          rewrite -IHidx; try lia.
+          f_equal.
+          rewrite /_set_byte.
+          rewrite !Z.shiftl_land.
+          apply Z.bits_inj'=> n ?.
+        +
+
+    Lemma _get_set_byte_roundtrip:
+      forall (v: Z) (idx: nat),
+        _get_byte (_set_byte v idx) idx = _get_byte v 0.
+    Proof.
+      move=> v idx; generalize dependent v;
+        induction idx; intros.
+      - rewrite /_get_byte/_set_byte/=.
+        cbv [Z.of_nat Z.mul];
+          rewrite ?Z.shiftr_0_r ?Z.shiftl_0_r;
+          try lia.
+        by rewrite Z.land_comm Z.land_assoc Z.land_diag Z.land_comm.
+      - rewrite _set_byte_S_idx _get_byte_S_idx
+                Z.shiftr_shiftl_r ?Z.sub_diag ?Z.shiftr_0_r;
+          try lia; apply IHidx.
+    Qed.
+
+    Lemma _set_get_byte_roundtrip:
+      forall (v: Z) (idx: nat),
+        _set_byte (_get_byte v idx) idx =
+        Z.land (Z.ones 8 ≪ (8 * idx)) v.
+    Proof.
+      rewrite /_get_byte/_set_byte=> v idx //=.
+      rewrite !Z.shiftl_land -Z.ldiff_ones_r; try lia.
+      apply Z.bits_inj' => n ?.
+      rewrite !Z.land_spec Z.ldiff_spec Z.shiftl_spec; try lia.
+      rewrite [Z.testbit (Z.ones (8 * idx)) n]Z.testbit_ones_nonneg; try lia.
+      destruct (n <? 8 * idx)%Z eqn:Hn;
+        rewrite ?andb_false_l ?andb_false_r
+                ?andb_true_l ?andb_true_r //.
+      - rewrite [Z.testbit (Z.ones 8) _]Z.testbit_neg_r
+                ?andb_false_l //.
+        apply Z.ltb_lt in Hn; lia.
+      - rewrite Z.testbit_ones_nonneg; try lia.
+        2: apply Z.ltb_ge in Hn; lia.
+        destruct (n - 8 * idx <? 8)%Z eqn:Hn';
+          rewrite ?andb_false_l ?andb_false_r
+                  ?andb_true_l ?andb_true_r //.
+    Qed.
+  End Theory.
+End Byte.
+
+Section Bswap.
+  #[local] Definition bswap_idxs (bytes: nat) :=
+    let idxs := seq 0 bytes in
+    zip idxs (rev idxs).
+
+  #[local] Definition bswap_ (bytes: nat) (n: Z): Z :=
+    fold_left (fun acc '(getIdx, setIdx) =>
+                 Z.lor acc (_set_byte (_get_byte n getIdx) setIdx))
+              (bswap_idxs bytes)
+              0.
+
+  #[local] Definition bswap16  (n: Z): Z := bswap_ 2 n.
+  #[local] Definition bswap32  (n: Z): Z := bswap_ 4 n.
+  #[local] Definition bswap64  (n: Z): Z := bswap_ 8 n.
+  #[local] Definition bswap128 (n: Z): Z := bswap_ 16 n.
+
+  Definition bswap (sz : bitsize) : Z -> Z :=
+    match sz with
+    | W8 => id
+    | W16 => bswap16
+    | W32 => bswap32
+    | W64 => bswap64
+    | W128 => bswap128
+    end.
+
+  Section Theory.
+    Section useless_lor.
+      Arguments Z.of_nat !_ /.
+      Arguments Z.opp !_ /.
+      Arguments Z.sub !_ !_ /.
+      Arguments Z.add !_ !_ /.
+      Arguments Z.mul !_ !_ /.
+      Arguments Pos.mul !_ !_ /.
+
+      Lemma bswap16_useless_lor:
+        forall v v' idx,
+          (idx >= 2)%nat ->
+          bswap16 (Z.lor v (_set_byte v' idx)) =
+          bswap16 v.
+      Proof.
+        move=> v v' idx Hidx.
+        rewrite /bswap16/bswap_/_get_byte/=.
+        rewrite !Z.lor_0_l !Z.shiftr_0_r.
+        1: f_equal; [ | do 1 (destruct idx; try lia)].
+        all: rewrite ?_set_byte_S_idx ?Z.shiftr_lor
+                     ?[Z.shiftl (Z.shiftl (_set_byte _ _) _) _]Z.shiftl_shiftl
+                     ?Z.shiftr_shiftl_l ?Z.land_lor_distr_l
+                     ?Z.sub_diag ?Z.shiftl_0_r
+                     ?(_set_byte_land_no_overlap idx 0) /=
+                     ?Z.shiftl_0_r ?Z.lor_0_r;
+          try lia.
+      Qed.
+
+      Lemma bswap32_useless_lor:
+        forall v v' idx,
+          (idx >= 4)%nat ->
+          bswap32 (Z.lor v (_set_byte v' idx)) =
+          bswap32 v.
+      Proof.
+        move=> v v' idx Hidx.
+        rewrite /bswap32/bswap_/_get_byte/=.
+        rewrite !Z.lor_0_l !Z.shiftr_0_r.
+        1: f_equal; [ | do 3 (destruct idx; try lia)].
+        1: f_equal; [ | do 2 (destruct idx; try lia)].
+        1: f_equal; [ | do 1 (destruct idx; try lia)].
+        all: rewrite ?_set_byte_S_idx ?Z.shiftr_lor
+                     ?[Z.shiftl (Z.shiftl (_set_byte _ _) _) _]Z.shiftl_shiftl
+                     ?Z.shiftr_shiftl_l ?Z.land_lor_distr_l
+                     ?Z.sub_diag ?Z.shiftl_0_r
+                     ?(_set_byte_land_no_overlap idx 0) /=
+                     ?Z.shiftl_0_r ?Z.lor_0_r;
+          try lia.
+      Qed.
+
+      Lemma bswap64_useless_lor:
+        forall v v' idx,
+          (idx >= 8)%nat ->
+          bswap64 (Z.lor v (_set_byte v' idx)) =
+          bswap64 v.
+      Proof.
+        move=> v v' idx Hidx.
+        rewrite /bswap64/bswap_/_get_byte/=.
+        rewrite !Z.lor_0_l !Z.shiftr_0_r.
+        1: f_equal; [ | do 7 (destruct idx; try lia)].
+        1: f_equal; [ | do 6 (destruct idx; try lia)].
+        1: f_equal; [ | do 5 (destruct idx; try lia)].
+        1: f_equal; [ | do 4 (destruct idx; try lia)].
+        1: f_equal; [ | do 3 (destruct idx; try lia)].
+        1: f_equal; [ | do 2 (destruct idx; try lia)].
+        1: f_equal; [ | do 1 (destruct idx; try lia)].
+        all: rewrite ?_set_byte_S_idx ?Z.shiftr_lor
+                     ?[Z.shiftl (Z.shiftl (_set_byte _ _) _) _]Z.shiftl_shiftl
+                     ?Z.shiftr_shiftl_l ?Z.land_lor_distr_l
+                     ?Z.sub_diag ?Z.shiftl_0_r
+                     ?(_set_byte_land_no_overlap idx 0) /=
+                     ?Z.shiftl_0_r ?Z.lor_0_r;
+          try lia.
+      Qed.
+
+    End useless_lor.
+
+    Section _set_byte_reverse.
+      Lemma bswap16_set_byte_reverse:
+        forall x1 x2,
+          bswap16 (Z.lor (_set_byte x1 0)
+                   (Z.lor (_set_byte x2 1) 0)) =
+          Z.lor (_set_byte x2 0)
+           (Z.lor (_set_byte x1 1) 0).
+      Proof.
+        move=> x1 x2.
+        rewrite /bswap16/bswap_/=.
+        rewrite !Z.lor_0_r !Z.lor_0_l.
+        rewrite {1}Z.lor_comm; f_equal.
+        - rewrite _get_byte_lor _set_byte_lor.
+          Set Nested Proofs Allowed.
+          Lemma _get_set_byte_no_overlap:
+            forall (v: Z) (idx idx': nat),
+              idx <> idx' ->
+              _get_byte (_set_byte v idx) idx' = 0.
+          Proof. Admitted.
+          rewrite _get_set_byte_no_overlap ?_set_byte_0 ?Z.lor_0_l; try lia.
+
+        - rewrite /_get_byte/_set_byte/=.
+          cbv [Z.of_nat Z.mul Pos.of_succ_nat Pos.mul]; rewrite !Z.shiftl_0_r.
+          rewrite ?Z.shiftl_land. rewrite ?Z.shiftr_land.
+          rewrite ?_set_byte_S_idx ?Z.shiftr_lor
+                  ?[Z.shiftl (Z.shiftl (_set_byte _ _) _) _]Z.shiftl_shiftl
+                  ?[Z.shiftr (Z.shiftl (_set_byte _ _) _) _]Z.shiftr_shiftl_l
+                  ?Z.land_lor_distr_l
+                  ?Z.sub_diag ?Z.shiftl_0_r
+                  ?(_set_byte_land_no_overlap idx 0) /=
+                  ?Z.shiftl_0_r ?Z.lor_0_r;
+            try lia.
+
+          rewrite Z.shiftr_shiftl_l.
+
+
+          apply Z.bits_inj' => n ?.
+          rewrite ?Z.land_spec ?Z.ldiff_spec ?Z.shiftl_spec; try lia.
+          rewrite [Z.testbit (Z.ones (8 * idx)) n]Z.testbit_ones_nonneg; try lia.
+          churn_bits.
+        -
+
+
+
+        rewrite _get_set_byte_roundtrip
+
+        rewrite /bswap16/bswap_/_get_byte/=.
+        cbv [Z.of_nat Z.mul Pos.of_succ_nat Pos.mul].
+        rewrite !Z.lor_0_r !Z.shiftr_0_r Z.lor_comm.
+        f_equal.
+        - rewrite ?_set_byte_S_idx ?Z.shiftr_lor
+                  ?[Z.shiftl (Z.shiftl (_set_byte _ _) _) _]Z.shiftl_shiftl
+                  ?[Z.shiftr (Z.shiftl (_set_byte _ _) _) _]Z.shiftr_shiftl_l
+                  ?Z.land_lor_distr_l
+                  ?Z.sub_diag ?Z.shiftl_0_r
+                  ?(_set_byte_land_no_overlap idx 0) /=
+                  ?Z.shiftl_0_r ?Z.lor_0_r;
+            try lia.
+          rewrite {1}[8]Zred_factor0 _set_byte_shiftr_big; try lia.
+          rewrite Z.land_0_l Z.lor_0_l.
+          rewrite _set_byte_land_useless;
+            [ | cbv [Z.of_nat Z.mul]; by rewrite Z.shiftl_0_r].
+          rewrite /_set_byte; cbv [Z.of_nat Z.mul]; rewrite !Z.shiftl_0_r.
+        -
+
+
+        - rewrite Z.shiftr_lor Z.land_lor_distr_l _set_byte_S_idx
+                  Z.shiftr_shiftl_l; try lia.
+          replace (8 - 8)%Z with 0%Z by lia.
+          rewrite Z.shiftl_0_r.
+          rewrite (_Z_set_byte_shiftr_big 0 1) ?Z.land_0_l ?Z.lor_0_l; try lia.
+          apply _Z_set_byte_land_useless.
+          by rewrite Z.shiftl_0_r.
+        - rewrite Z.land_lor_distr_l.
+          rewrite (_Z_set_byte_land_no_overlap 1 0);
+            [
+            | by lia
+            | by rewrite Z.shiftl_0_r];
+            rewrite Z.lor_0_r.
+          rewrite _Z_set_byte_land_useless;
+            [
+            | by rewrite Z.shiftl_0_r].
+          by rewrite -_Z_set_byte_S_idx.
+      Qed.
+
+    End _set_byte_reverse.
+
+  End Theory.
+
+  Section test.
+    Local Definition bytes (ls : list Z) :=
+      fold_left (fun a b => a * 256 + b)%Z ls 0%Z.
+    Arguments bytes _%Z.
+
+    Local Definition _bswap16_test : bswap W16 (bytes (1::2::nil)%Z) = bytes (2::1::nil)%Z := eq_refl.
+    Local Definition _bswap32_test :
+      bswap W32 (bytes (1::2::3::4::nil)%Z) = bytes (4::3::2::1::nil)%Z := eq_refl.
+    Local Definition _bswap64_test :
+      bswap W64 (bytes (1::2::3::4::5::6::7::8::nil)%Z) = bytes (8::7::6::5::4::3::2::1::nil)%Z := eq_refl.
+  End test.
+End bswap.
